allow `const` source buffers for memcpy
this commit should go hand-in-hand with FStarLang/karamel#537

lib/pulse/lib/Pulse.Lib.ArrayPtr.fst
@@ -227,37 +227,3 @@ fn join (#t: Type) (s1: ptr t) (#p: perm) (#v1: Seq.seq t) (s2: ptr t) (#v2: Seq
     A.pts_to_range_join s1.base (SZ.v s1.offset) (SZ.v s1.offset + Seq.length v1) (SZ.v s1.offset + Seq.length v1 + Seq.length v2);
     fold_pts_to s1 #p (Seq.append v1 v2)
 }
-
-module R = Pulse.Lib.Reference
-
-fn memcpy
-    (#t:Type0) (#p0:perm)
-    (src:ptr t) (idx_src: SZ.t)
-    (dst:ptr t) (idx_dst: SZ.t)
-    (len: SZ.t)
-    (#s0:Ghost.erased (Seq.seq t) { SZ.v idx_src + SZ.v len <= Seq.length s0 })
-    (#s1:Ghost.erased (Seq.seq t) { SZ.v idx_dst + SZ.v len <= Seq.length s1 })
-  requires pts_to src #p0 s0 ** pts_to dst s1
-  ensures pts_to src #p0 s0 **
-    pts_to dst (Seq.slice s0 0 (SZ.v len) `Seq.append` Seq.slice s1 (SZ.v len) (Seq.length s1))
-{
-  let mut i = 0sz;
-  while (let vi = !i; SZ.lt vi len)
-    invariant b. exists* s1' vi.
-      R.pts_to i vi **
-      pts_to src #p0 s0 **
-      pts_to dst s1' **
-      pure (b == SZ.lt vi len /\ SZ.lte vi len /\
-        Seq.length s1' == Seq.length s1 /\
-        forall (j:nat). j < Seq.length s1' ==>
-          Seq.index s1' j == (if j < SZ.v vi then Seq.index s0 j else Seq.index s1 j))
-  {
-    let vi = !i;
-    let x = src.(vi);
-    dst.(vi) <- x;
-    i := SZ.add vi 1sz;
-  };
-  with s1'. assert pts_to dst s1';
-  assert pure (s1' `Seq.equal`
-    (Seq.slice s0 0 (SZ.v len) `Seq.append` Seq.slice s1 (SZ.v len) (Seq.length s1)))
-}
