lib/pulse/lib/Pulse.Lib.ConstArrayPtr.fst
@@ -45,3 +45,37 @@ let split #t s #p i #v = AP.split #t s #p i #v
 let ghost_split #t s #p i #v = AP.ghost_split #t s #p i #v
 
 let join #t s1 #p #v1 s2 #v2 = AP.join #t s1 #p #v1 s2 #v2
+
+module R = Pulse.Lib.Reference
+
+fn memcpy
+    (#t:Type0) (#p0:perm)
+    (src:ptr t) (idx_src: SZ.t)
+    (dst:ptr t) (idx_dst: SZ.t)
+    (len: SZ.t)
+    (#s0:Ghost.erased (Seq.seq t) { SZ.v idx_src + SZ.v len <= Seq.length s0 })
+    (#s1:Ghost.erased (Seq.seq t) { SZ.v idx_dst + SZ.v len <= Seq.length s1 })
+  requires pts_to src #p0 s0 ** pts_to dst s1
+  ensures pts_to src #p0 s0 **
+    pts_to dst (Seq.slice s0 0 (SZ.v len) `Seq.append` Seq.slice s1 (SZ.v len) (Seq.length s1))
+{
+  let mut i = 0sz;
+  while (let vi = !i; SZ.lt vi len)
+    invariant b. exists* s1' vi.
+      R.pts_to i vi **
+      pts_to src #p0 s0 **
+      pts_to dst s1' **
+      pure (b == SZ.lt vi len /\ SZ.lte vi len /\
+        Seq.length s1' == Seq.length s1 /\
+        forall (j:nat). j < Seq.length s1' ==>
+          Seq.index s1' j == (if j < SZ.v vi then Seq.index s0 j else Seq.index s1 j))
+  {
+    let vi = !i;
+    let x = src.(vi);
+    AP.op_Array_Assignment dst vi x;
+    i := SZ.add vi 1sz;
+  };
+  with s1'. assert pts_to dst s1';
+  assert pure (s1' `Seq.equal`
+    (Seq.slice s0 0 (SZ.v len) `Seq.append` Seq.slice s1 (SZ.v len) (Seq.length s1)))
+}
