lib/pulse/lib/Pulse.Lib.ConstArrayPtr.fsti
@@ -119,3 +119,14 @@ val ghost_split (#t: Type) (s: ptr t) (#p: perm) (i: SZ.t)
 val join (#t: Type) (s1: ptr t) (#p: perm) (#v1: Seq.seq t) (s2: ptr t) (#v2: Seq.seq t) : stt_ghost unit emp_inames
     (pts_to s1 #p v1 ** pts_to s2 #p v2 ** pure (adjacent s1 (Seq.length v1) s2))
     (fun _ -> pts_to s1 #p (Seq.append v1 v2))
+
+val memcpy
+    (#t:Type0) (#p0:perm)
+    (src:ptr t) (idx_src: SZ.t)
+    (dst:AP.ptr t) (idx_dst: SZ.t)
+    (len: SZ.t)
+    (#s0:Ghost.erased (Seq.seq t) { SZ.v idx_src + SZ.v len <= Seq.length s0 })
+    (#s1:Ghost.erased (Seq.seq t) { SZ.v idx_dst + SZ.v len <= Seq.length s1 })
+  : stt unit
+    (pts_to src #p0 s0 ** pts_to dst s1)
+    (fun _ -> pts_to src #p0 s0 ** pts_to dst (Seq.slice s0 0 (SZ.v len) `Seq.append` Seq.slice s1 (SZ.v len) (Seq.length s1)))
